unbundle invGS_gen from melocotonGS
This makes it possible to work with two different languages and their
WPs, sharing the same notion of logical invariant (and fancy update,
etc). Previously, each language would come with its (possibly
incompatible) invGS_gen instance, resulting in two (incompatible)
ghost state for invariants being in scope.

NB: for mlanguage, invGS_gen is already unbundled from mlangGS, for
the same reasons.

theories/c_toy_lang/melocoton/primitive_laws.v
@@ -10,8 +10,7 @@ From melocoton.c_toy_lang Require Export melocoton.class_instances.
 From melocoton.c_toy_lang Require Import tactics melocoton.tactics notation.
 From iris.prelude Require Import options.
 
-Class heapGS_C_gen hlc Σ := HeapGS {
-  heapGS_invGS : invGS_gen hlc Σ;
+Class heapGS_C Σ := HeapGS {
   heapGS_gen_heapGS :> gen_heapGS loc heap_cell Σ;
   heapGS_inv_heapGS :> inv_heapGS loc heap_cell Σ;
   heapGS_proph_mapGS :> proph_mapGS positive (prod val val) Σ;
@@ -20,10 +19,8 @@ Class heapGS_C_gen hlc Σ := HeapGS {
 }.
 Local Existing Instance heapGS_step_cnt.
 
-Notation heapGS_gen := (heapGS_C_gen).
-
 Section steps.
-  Context `{!heapGS_gen hlc Σ}.
+  Context `{!heapGS_C Σ}.
 
   Local Definition steps_auth (n : nat) : iProp Σ :=
     mono_nat_auth_own heapGS_step_name 1 n.
@@ -59,14 +56,13 @@ Section steps.
 
 End steps.
 
-Global Program Instance heapGS_melocotonGS_C `{heapGS_gen hlc Σ} 
-      : melocotonGS_gen hlc val C_lang Σ := {
-  iris_invGS := heapGS_invGS;
+Global Program Instance heapGS_melocotonGS_C `{heapGS_C Σ}
+      : melocotonGS val C_lang Σ := {
   state_interp σ step_cnt :=
     (gen_heap_interp σ ∗ steps_auth step_cnt)%I
 }.
 Next Obligation.
-  iIntros (??? σ ns E)  "/= ($ & H)".
+  iIntros (???? σ ns E)  "/= ($ & H)".
   by iMod (steps_auth_update_S with "H") as "$".
 Qed.
 
@@ -114,7 +110,7 @@ Notation "l ↦C '?'" := (mapsto (L:=loc) (V:=heap_cell) l (DfracOwn 1) (Uniniti
 make setoid rewriting in the predicate [I] work we need actual definitions
 here. *)
 Section definitions.
-  Context `{!heapGS_gen hlc Σ}.
+  Context `{!heapGS_C Σ}.
 
   Definition from_storing (I : val → Prop) (Puninit Pfree : Prop) (k : heap_cell) :=
     match k with
@@ -139,7 +135,7 @@ Notation "l ↦_ I v" := (inv_mapsto_own l v I%stdpp%type)
   (at level 20, I at level 9, format "l  ↦_ I  v") : bi_scope.
 
 Section lifting.
-Context `{!heapGS_gen hlc Σ}.
+Context `{!heapGS_C Σ, !invGS_gen hlc Σ}.
 Context {p:prog_environ C_lang Σ}.
 Implicit Types P Q : iProp Σ.
 Implicit Types Φ Ψ : val → iProp Σ.
