theories/c_toy_lang/melocoton/derived_laws.v
@@ -14,7 +14,7 @@ From iris.prelude Require Import options.
 (** The [array] connective is a version of [mapsto] that works
 with lists of values. *)
 
-Definition array `{!heapGS_gen hlc Σ} (l : loc) (dq : dfrac) (vs : list (option val)) : iProp Σ :=
+Definition array `{!heapGS_C Σ} (l : loc) (dq : dfrac) (vs : list (option val)) : iProp Σ :=
   [∗ list] i ↦ v ∈ vs, (l +ₗ i) I↦{dq} v.
 
 (** FIXME: Refactor these notations using custom entries once Coq bug #13654
@@ -33,8 +33,7 @@ Notation "l ↦∗ vs" := (array l (DfracOwn 1) vs)
 lead to overlapping instances. *)
 
 Section lifting.
-Notation heapGS_gen := (heapGS_C_gen).
-Context `{!heapGS_gen hlc Σ}.
+Context `{!heapGS_C Σ, !invGS_gen hlc Σ}.
 Context {p:program}.
 Implicit Types P Q : iProp Σ.
 Implicit Types Φ : val → iProp Σ.
